Cleanup and some documentation

theory/cwp/geometric.v
@@ -12,57 +12,15 @@ Require Import Q.
 
 Fixpoint geometric_series (a r : Q) (n : nat) :=
   match n with
-  | O => a
-  | S n' => geometric_series a r n' + a * Qpow r n
-  end.
-
-(** This is the one being used currently. *)
-Fixpoint geometric_series'' (a r : Q) (n : nat) :=
-  match n with
   | O => 0
-  | S n' => geometric_series'' a r n' + a * Qpow r n'
+  | S n' => geometric_series a r n' + a * Qpow r n'
   end.
 
-(** This slightly different series is used instead for wlp. *)
+(** This slightly different series is used instead for wlp. It
+  includes an additional term that is large initially but converges to
+  zero as n increases. *)
 Definition wlpf_series (a r : Q) (n : nat) :=
-  geometric_series'' a r n + Qpow r n.
-
-Definition geometric_series' (a r : Q) (n : nat) : Q :=
-  sum_Q_list (map (fun n => a * Qpow r n) (seq O (S n))).
-
-Lemma geometric_series_geometric_series' (a r : Q) (n : nat) :
-  geometric_series a r n == geometric_series' a r n.
-Proof.
-  unfold geometric_series'.
-  induction n.
-  - simpl; field.
-  - simpl in *.
-    rewrite IHn. ring_simplify.
-    set (f := fun n => a * Qpow r n).
-    assert (a == f O).
-    { unfold f. simpl. field. }
-    rewrite H, <- Qplus_assoc, sum_Q_list_l, Qplus_comm; simpl.
-    assert (H0: f O * r * Qpow r n == f (1 + n)%nat).
-    { unfold f. simpl. field. }
-    rewrite H0, <- Qplus_assoc, sum_Q_list_r.
-    unfold f; simpl; field.
-Qed.
-
-Lemma geometric_series_geometric_series'' (a r : Q) (n : nat) :
-  geometric_series a r n == geometric_series'' a r (S n).
-Proof.
-  induction n; simpl.
-  - lra.
-  - rewrite IHn; reflexivity.
-Qed.
-
-Lemma geometric_series_cons_geometric_series'' (a r : Q) (n : nat) :
-  cons_chain 0 (geometric_series a r) n == geometric_series'' a r n.
-Proof.
-  destruct n.
-  - reflexivity.
-  - apply geometric_series_geometric_series''.
-Qed.
+  geometric_series a r n + Qpow r n.
 
 Definition pow_series (a : Q) (i : nat) := Qpow a i.
 
@@ -74,36 +32,10 @@ Axiom geometric_series_converges :
     0 <= r -> r < 1 ->
     converges (geometric_series a r) (a / (1 - r)).
 
-Axiom geometric_series''_converges :
-  forall a r,
-    0 <= r -> r < 1 ->
-    converges (geometric_series'' a r) (a / (1 - r)).
-
 Axiom pow_series_converges :
   forall a,
     0 <= a -> a < 1 ->
     converges (pow_series a) 0.
-
-
-(* Definition converges_from_below (g : nat -> Q) (lim : Q) := *)
-(*   forall eps, 0 < eps -> *)
-(*          exists n0, forall n, *)
-(*              (n0 <= n)%nat -> lim - g n < eps. *)
-
-(* Axiom geometric_series_converges : *)
-(*   forall a r, converges (geometric_series a r) (a / (1 - r)). *)
-
-(* Axiom geometric_series_converges : *)
-(*   forall a r eps, *)
-(*     0 <= a <= 1 -> 0 <= r -> r < 1 -> 0 < eps -> *)
-(*     exists n0, forall n, *)
-(*         (n0 <= n)%nat -> (a / (1 - r)) - geometric_series a r n < eps. *)
-
-(* Definition prefix_series {A : Type} (n : nat) (f : nat -> A) (i : nat) := *)
-(*   f (i-n)%nat. *)
-
-(* Definition postfix_series {A : Type} (n : nat) (f : nat -> A) (i : nat) := *)
-(*   f (i-n)%nat. *)
 
 Lemma sum_converges f g limf limg :
   converges f limf /\ converges g limg ->
@@ -138,61 +70,26 @@ Lemma wlpf_series_converges :
     converges (wlpf_series a r) (a / (1 - r)).
 Proof.
   intros a r Hle Hlt.
-  set (f := (geometric_series'' a r)).
+  set (f := (geometric_series a r)).
   set (g := fun i => Qpow r i).
   cut (converges (fun i => f i + g i) (a / (1 - r) + 0)).
   - intro Hc; eapply Proper_converges; eauto. reflexivity. lra.
   - apply sum_converges. split.
-    + apply geometric_series''_converges; auto.
+    + apply geometric_series_converges; auto.
     + apply pow_series_converges; auto.
 Qed.
 
 Lemma geometric_series_succ (a r : Q) (n : nat) :
   a + r * geometric_series a r n == geometric_series a r (S n).
 Proof.
-  rewrite 2!geometric_series_geometric_series'.
-  unfold geometric_series'. simpl.
-  set (f := fun i => a * Qpow r i).
-  assert (H0: a * 1 == f O).
-  { reflexivity. }
-  rewrite H0.
-  rewrite sum_Q_list_l.
-  assert (H1: a * (r * 1) == f (S O)).
-  { reflexivity. }
-  rewrite H1.
-  rewrite sum_Q_list_l. rewrite sum_Q_list_l.
-  rewrite sum_Q_list_distr. unfold f.
-  rewrite sum_Q_list_Qpow; simpl; field.
-Qed.
-
-Lemma geometric_series''_succ (a r : Q) (n : nat) :
-  a + r * geometric_series'' a r n == geometric_series'' a r (S n).
-Proof.
-  rewrite <- geometric_series_geometric_series''.
   induction n; simpl.
   - lra.
-  - rewrite <- IHn; lra.
+  - rewrite Qmult_plus_distr_r, Qplus_assoc, IHn; simpl; lra.
 Qed.
 
 Lemma geometric_series_monotone (a r : Q) :
   0 <= a -> 0 <= r ->
   monotone (geometric_series a r).
-Proof.
-  intros Hle_a Hle_r n m Hleq. simpl in *.
-  induction m. simpl.
-  - inversion Hleq; subst; simpl; lra.
-  - unfold Nat.le in *.
-    destruct (Nat.eqb_spec n (S m)); subst. lra.
-    assert (Hle: (n <= m)%nat). lia.
-    apply IHm in Hle. simpl.
-    generalize (@Qpow_nonnegative r m Hle_r).
-    intro Hle_pow.
-    assert (0 <= r * Qpow r m); nra.
-Qed.
-
-Lemma geometric_series''_monotone (a r : Q) :
-  0 <= a -> 0 <= r ->
-  monotone (geometric_series'' a r).
 Proof.
   intros Hle_a Hle_r n m Hleq. simpl in *.
   induction m. simpl.
@@ -293,29 +190,21 @@ Qed.
 
 Lemma geometric''_supremum (ch : nat -> Q) (a r : Q) :
   0 <= a -> 0 <= r -> r < 1 ->
-  ch ==f geometric_series'' a r ->
+  ch ==f geometric_series a r ->
   supremum (a / (1 - r)) ch.
 Proof.
   intros Hle_a Hle_r0 Hle_r1 Heq.
   apply converges_from_below_supremum.
   - intro i. unfold f_Qeq in Heq. rewrite 2!Heq.
-    apply geometric_series''_monotone; auto; simpl; unfold Nat.le; lia.
+    apply geometric_series_monotone; auto; simpl; unfold Nat.le; lia.
   - eapply Proper_converges; eauto. reflexivity.
-    apply geometric_series''_converges; auto.
+    apply geometric_series_converges; auto.
 Qed.
 
 Instance Proper_geometric_series
   : Proper (Qeq ==> Qeq ==> eq ==> Qeq) geometric_series.
 Proof.
   intros a b Heq1 c d Heq2 n m Heq3.
-  subst. induction m; simpl; auto.
+  subst. induction m; simpl; auto; try reflexivity.
   rewrite IHm, Heq1, Heq2; reflexivity.
-Qed.
-
-Lemma geometric_series_const (a : Q) (n : nat) :
-  geometric_series a 0 n == a.
-Proof.
-  induction n; simpl.
-  - reflexivity.
-  - rewrite IHn; lra.
 Qed.
