theory/cwp/cpGCL.v
@@ -1,13 +1,16 @@
-(** The cpGCL language and associated definitions. *)
+(** The conditional probabilistic guarded command language (cpGCL). *)
 
 Require Import Coq.Program.Basics.
 Require Import Coq.QArith.QArith.
 
+(** For now we support only boolean values. *)
 Definition val := bool.
+(** A program state is a map from identifiers (nat) to values. *)
 Definition St : Type := nat -> val.
 Definition empty : St := fun _ => false.
 Definition upd (x : nat) (v : val) (st : St) : St :=
   fun y => if Nat.eqb y x then v else st y.
+(** An expression is a function from program states to values. *)
 Definition exp := St -> val.
 
 Inductive cpGCL : Type :=
@@ -27,8 +30,10 @@ Record prog :=
 Notation "a ';;' b" := (CSeq a b) (at level 100, right associativity) : cpGCL_scope.
 Open Scope cpGCL_scope.
 
-(* TODO: restrictions on reading/writing to variables within
-   while-loops to ensure correctness of tree inference. *)
+(** A cpGCL command is well-formed when all p values in choice
+    commands are valid probabilities. *)
+(** NOTE: this could be strengthened to [0 < p < 1] since choice
+    commands with p=0 or p=1 are unnecessary and can be eliminated. *)
 Inductive wf_cpGCL : cpGCL -> Prop :=
 | wf_skip : wf_cpGCL CSkip
 | wf_abort : wf_cpGCL CAbort
@@ -46,68 +51,5 @@ Inductive wf_cpGCL : cpGCL -> Prop :=
 (** f is an expectation. *)
 Definition expectation {A : Type} (f : A -> Q) := forall x, 0 <= f x.
 
-(** f is a bounded expectation. *)
+(** f is a bounded expectation (bounded above by 1). *)
 Definition bounded_expectation {A : Type} (f : A -> Q) := forall x, 0 <= f x <= 1.
-
-(* Require Import FunctionalExtensionality. *)
-
-(* Lemma kjfg (e e0 : exp) n x : *)
-(*   e (upd n (e0 (upd n (e0 x) x)) (upd n (e0 x) x)) = *)
-(*   e (upd n (e0 x) x). *)
-(* Proof. *)
-(*   f_equal. apply functional_extensionality; intro y. *)
-(*   unfold upd.  *)
-(*   destruct (Nat.eqb_spec y n). *)
-
-(* Lemma upd_twice (n : nat) (e : exp) (x : St) : *)
-(*   (upd n (e (upd n (e x) x)) x) = (upd n (e x) x). *)
-(* Proof. *)
-(*   apply functional_extensionality; intro y. *)
-(*   destruct (e x). unfold upd. *)
-(*   destruct (Nat.eqb_spec y n); subst; auto. *)
-(* Qed. *)
-
-(* Lemma jkdfgdf (f : bool -> bool) : *)
-(*   f = const false \/ f = const true \/ f = id \/ f = negb. *)
-(* Proof. *)
-(*   destruct (f false) eqn:Hf; destruct (f true) eqn:Ht. *)
-(*   - right; left; apply functional_extensionality; intros []; auto. *)
-(*   - right; right; right; apply functional_extensionality; intros []; auto. *)
-(*   - right; right; left; apply functional_extensionality; intros []; auto. *)
-(*   - left; apply functional_extensionality; intros []; auto. *)
-(* Qed. *)
-
-(* Local Open Scope program_scope. *)
-(* Lemma bool_involutive (f : bool -> bool) : *)
-(*   (exists c, f = const c) \/ f ∘ f = id. *)
-(* Proof. *)
-(*   unfold compose, const. *)
-(*   destruct (jkdfgdf f) as [H|[H|[H|H]]]; subst. *)
-(*   - left; exists false; auto. *)
-(*   - left; exists true; auto. *)
-(*   - right; reflexivity. *)
-(*   - right. apply functional_extensionality; intros []; auto. *)
-(* Qed. *)
-
-(* (* Lemma upd_twice (n : nat) (e : exp) (x : St) : *) *)
-(* (*   e (upd n () x) *) *)
-(* (* Proof. *) *)
-(* (*   apply functional_extensionality; intro y. *) *)
-(* (*   destruct (e x). unfold upd. *) *)
-(* (*   destruct (Nat.eqb_spec y n); subst; auto. *) *)
-(* (* Qed. *) *)
-
-(* Lemma upd_shadow n st z y : *)
-(*   upd n y (upd n z st) = upd n y st. *)
-(* Proof. *)
-(*   apply functional_extensionality; intro x. *)
-(*   unfold upd. destruct (Nat.eqb_spec x n); subst; reflexivity. *)
-(* Qed. *)
-
-(* (* Lemma upd_ext (st1 st2 : St) (e : exp) : *) *)
-(* (*   (forall x, st1 x = st2 x) -> *) *)
-(* (*   e st1 = e st2. *) *)
-(* (* Proof. *) *)
-(* (*   apply functional_extensionality in  *) *)
-(* (*   intro Heq.  *) *)
-(* (* Qed. *) *)
